GTD, RW

examples/layeredeffects/RW.fst
@@ -1,102 +1,150 @@
 module RW
 
+#set-options "--print_effect_args"
+
 module H = FStar.Heap
 open FStar.Tactics
 open FStar.Universe
 open FStar.ST
 
 type idx =
- | R
- //| W
+ | RO
  | RW
-
-// GM: Force a type equality by SMT
-let coerce #a #b (x:a{a == b}) : b = x
-
-let m (a:Type u#aa) (i:idx) : Type0 =
-  match i with
-  | R  -> (unit -> ST a (requires (fun _ -> True)) (ensures (fun h0 _ h1 -> h0 == h1)))
-  //| W  -> unit -> ST a (requires (fun _ -> True)) (ensures (fun _ _ _ -> True))
-  | RW -> unit -> ST a (requires (fun _ -> True)) (ensures (fun _ _ _ -> True))
-
-let return_r  #a (x:a) : m a R  = fun () -> x
-let return_rw #a (x:a) : m a RW = fun () -> x
-
-let reveal_r #a (f : m a R) : (unit -> ST a (requires (fun _ -> True)) (ensures (fun h0 _ h1 -> h0 == h1))) =
-  f
-  
-let reveal_rw #a (f : m a RW) : (unit -> ST a (requires (fun _ -> True)) (ensures (fun _ _ _ -> True))) =
-  f
-  
-let pack_r #a (f : unit -> ST a (requires (fun _ -> True)) (ensures (fun h0 _ h1 -> h0 == h1))) : m a R =
-  f
-  
-let pack_rw #a (f : (unit -> ST a (requires (fun _ -> True)) (ensures (fun _ _ _ -> True)))) : m a RW =
-  f
-
-let return (a:Type) (x:a) (i:idx) : m a i =
-  match i with
-  | R  -> return_r x
-  | RW -> return_rw x
-
-let bind_r #a #b ($c : m a R) ($f : a -> m b R) : m b R = fun () -> f (c ()) ()
-let bind_rw #a #b ($c : m a RW) ($f : a -> m b RW) : m b RW = fun () -> f (c ()) ()
-
-let bind (a b : Type) (i:idx) (c : m a i) (f : a -> m b i) : m b i =
-  match i with
-  | R  -> coerce (bind_r #a #b c f)
-  | RW -> coerce (bind_rw #a #b c f)
-
-// Already somewhat usable
-let rec r_map #i #a #b (f : a -> m b i) (xs : list a) : m (list b) i =
-  match xs with
-  | [] -> return _ [] _
-  | x::xs ->
-    bind _ _ _ (f x) (fun y ->
-    bind _ _ _ (r_map f xs) (fun ys ->
-    return _ (y::ys) _))
-
+ 
 // cannot make this prop
 val flows : idx -> idx -> Type0
 let flows i1 i2 =
   match i1, i2 with
-  | RW, R -> False
+  | RW, RO -> False
   | _, _ -> True
 
-// fails with ref
+// fails later if we use this refinement
 //val join : i1:idx -> i2:idx -> r:idx{flows i1 r /\ flows i2 r}
 val join : i1:idx -> i2:idx -> idx
 let join i1 i2 =
   match i1, i2 with
-  | R, R -> R
+  | RO, RO -> RO
   | _, _ -> RW
 
-let subcomp (a:Type) (i1 i2 :idx) (f : m a i1) : Pure (m a i2)
-                                                      (requires (flows i1 i2))
-                                                      (ensures (fun _ -> True))
-  = match i1, i2 with
-    | R, R -> coerce f
-    | RW, RW -> coerce f
-    | R, RW -> 
-      let f' () : ST a (fun _ -> True) (fun _ _ _ -> True) = reveal_r f () in
-      f'
+// GM: Force a type equality by SMT
+let coerce #a #b (x:a{a == b}) : b = x
 
+// unfold
+// let rowp #a (wp : st_wp a) : st_wp a =
+//   fun p h0 -> wp (fun x h1 -> h0 == h1 ==> p x h1) h0
+// 
+// let st_monotonic #a (wp : st_wp a) : Type =
+//   forall p1 p2 h0. (forall x h1. p1 x h1 ==> p2 x h1) ==> wp p1 h0 ==> wp p2 h0
+// 
+// let test_ro
+//   (#wp:_{st_monotonic wp})
+//   (f : unit -> STATE int (rowp wp))
+// : ST int (fun h0 -> wp (fun _ _ -> True) h0) (fun _ _ _ -> True)
+// = let h0 = get ()in
+//   let _ = f () in
+//   let h1 = get ()in
+//   assert (h0 == h1);
+//   42
 
-#set-options "--debug RW --debug_level SMTQuery"
+// this can be seen as a lifting from RO postconditions to RW postconditions
+unfold
+let ro_post #a (post : H.heap -> st_post a) : H.heap -> st_post a =
+  fun h0 x h1 -> post h0 x h1 /\ h1 == h0
 
-// GM: I'm surprised this works, I thought we had the req that
-//
-//    p ==> if_then_else _ _ _ f1 f2 = (typeof f1)
-//
-// but that's not true since the join can raise the index... unless the _ are solved to
-// the same index? is that ok?
-let if_then_else (a:Type) (i1 i2:idx) (f : m a i1) (g : m a i2) (p : Type0) : Type =
-  m a (join i1 i2)
+let is_ro_post #a (post : H.heap -> st_post a) : Type =
+  forall h0 x h1. post h0 x h1 ==> h0 == h1
+
+let st_bpost (a:Type) : Type =
+  H.heap -> a -> H.heap -> Type0
+  
+let ro_sanity_check #a (post : H.heap -> st_post a) =
+  assert (is_ro_post (ro_post post))
+
+let real_post #a (i : idx) (post : st_bpost a)
+  : st_bpost a
+  = match i with
+    | RO -> ro_post post
+    | _ -> post
+  
+// GM: Note, postconditions are totally defined, their well-typing cannot
+// depend on pre (see issue #57 and the `st_post'` type).
+let m (a:Type u#aa) (i:idx) (pre : st_pre) (post : st_bpost a): Type0 =
+  unit -> ST a pre (real_post i post)
+  
+let return (a:Type) (x:a) : m a RO (fun _ -> True) (fun h0 y h1 -> y == x /\ h1 == h0) =
+  fun () -> x
+
+unfold
+let bind_pre #a (i1 i2 : idx)
+  (pre : st_pre)
+  (pre' : a -> st_pre)
+  (post : st_bpost a)
+  : st_pre
+  = let post = real_post i1 post in
+    fun h0 -> pre h0 /\ (forall x h1. post h0 x h1 ==> pre' x h1)
+    
+unfold
+let bind_post #a #b (i1 i2 : idx)
+  (pre : st_pre)
+  (post : st_bpost a)
+  (post' : a -> st_bpost b)
+  : st_bpost b
+  = let post    : st_bpost a = real_post i1 post in
+    let post' x : st_bpost b = real_post i2 (post' x) in
+    fun h0 y h2 -> pre h0 /\ (exists x h1. post h0 x h1 /\ post' x h1 y h2)
+
+let bind (a b : Type)
+  (i i' :idx)
+  (pre:_) (post:st_bpost a)
+  (pre':_) (post':a -> st_bpost b)
+  (c : m a i pre post)
+  (f : (x:a -> m b i' (pre' x) (post' x)))
+  : Tot (m b (join i i') (bind_pre i i' pre pre' post) (bind_post i i' pre post post'))
+  = fun () -> let x = c () in f x ()
+
+// a test
+let rwi_subtype (a b : Type) (inj : a -> b)
+  (i:idx)
+  (pre:_) (post:st_bpost a)
+  (c : m a i pre post)
+  : Tot (m b i pre (fun h0 x h1 -> exists x0. x == inj x0 /\ post h0 x0 h1)) =
+  bind _ _ _ _ _ _ _ _ c (fun (x:a) -> return _ (inj x))
+
+let pre_leq (pre1 pre2 : st_pre) =
+  forall h. pre2 h ==> pre1 h
+
+let post_leq #a (post1 post2 : H.heap -> st_post a) =
+  forall h0 x h1. post1 h0 x h1 ==> post2 h0 x h1
+
+// how is subtyping handled? can I subtype on a?
+// note that post is contravariant in a
+let subcomp (a:Type) (i1 i2 :idx)
+  (pre : st_pre)  (post  : st_bpost a)
+  (pre' : st_pre) (post' : st_bpost a)
+  (f : m a i1 pre post)
+  : Pure (m a i2 pre' post')
+         (requires (flows i1 i2 /\ pre_leq pre pre' /\ post_leq post post'))
+         (ensures (fun _ -> True))
+  = fun () -> f ()
+  
+let ite (p q r : Type0) = (p ==> q) /\ (~p ==> r)
+
+let if_then_else
+  (a : Type) (i1 i2 : idx)
+  (pre1 pre2 : st_pre)
+  (post1 : st_bpost a)
+  (post2 : st_bpost a)
+  (f : m a i1 pre1 post1) (g : m a i2 pre2 post2)
+  (p : Type0)
+  : Type
+  = m a (join i1 i2)
+        (fun h0 -> ite p (pre1 h0) (pre2 h0))
+        (fun h0 x h1 -> ite p (post1 h0 x h1) (post2 h0 x h1))
 
 reifiable
 reflectable
 layered_effect {
-  RWI : a:Type -> idx -> Effect
+  RWI : a:Type -> i:idx -> st_pre -> st_bpost a  -> Effect
   with
   repr         = m;
   return       = return;
@@ -105,77 +153,159 @@ layered_effect {
   if_then_else = if_then_else
 }
 
-let lift_pure_rwi (a:Type) (wp : pure_wp a) (i : idx)
-                  (f : unit -> PURE a wp)
-                 : Pure (m a i)
-                        (requires (wp (fun _ -> True) /\ (forall p1 p2. (forall x. p1 x ==> p2 x) ==> wp p1 ==> wp p2)))
-                        (ensures (fun _ -> True))
- =
- match i with
- | R ->
-   let f' () : ST a (fun _ -> True) (fun h0 _ h1 -> h0 == h1) = f () in
-   f'
- | RW ->
-   let f' () : ST a (fun _ -> True) (fun h0 _ h1 -> True) = f () in
-   f'
+unfold
+let pure_monotonic #a (wp : pure_wp a) : Type =
+  forall p1 p2. (forall x. p1 x ==> p2 x) ==> wp p1 ==> wp p2
 
+unfold
+let sp #a (wp : pure_wp a) : pure_post a =
+  fun x -> ~ (wp (fun y -> ~(x == y)))
+
+let lift_pure_rwi
+ (a:Type)
+ (wp : pure_wp a)
+ (f : unit -> PURE a wp)
+ // with the index-polymorphic bind above, this has to be in RO,
+ // or unification will usually not find the index here
+ : Pure (m a RO (fun _ -> wp (fun _ -> True)) (fun h0 x h1 -> sp wp x /\ h1 == h0))
+        (requires pure_monotonic wp)
+        (ensures (fun _ -> True))
+ = fun () -> f ()
+ 
 sub_effect PURE ~> RWI = lift_pure_rwi
 
-// cannot resolve an index
+let test_rrr #pre #post (b:bool) (f : unit -> RWI int RO pre post) (g : unit -> RWI int RO pre post) : RWI int RO pre post = if b then f () else g ()
+
+let test_rrw #pre #post (b:bool) (f : unit -> RWI int RO pre post) (g : unit -> RWI int RO pre post) : RWI int RW pre post = if b then f () else g ()
+
 [@@expect_failure]
-let rec map #a #b (#i:idx) (f : a -> RWI b i) (xs : list a) : RWI (list b) i =
-  match xs with
-  | [] -> []
-  | x::xs -> (f x)::(map #_ #_ #i f xs)
+let test_rwr #pre #post (b:bool) (f : unit -> RWI int RO pre post) (g : unit -> RWI int RW pre post) : RWI int RO pre post = if b then f () else g ()
 
-let app #a #b #i (f : a -> RWI b i) (x : a) : RWI b i = f x
+let test_rww #pre #post (b:bool) (f : unit -> RWI int RO pre post) (g : unit -> RWI int RW pre post) : RWI int RW pre post = if b then f () else g ()
 
-// also can't resolve an index
 [@@expect_failure]
-let rec appn #a #i (n:nat) (f : a -> RWI a i) (x : a) : RWI a i =
-  match n with 
-  | 0 -> x
-  | _ -> begin
-    assume (n>0);
-    appn (n-1) f (f x)
-  end
+let test_wrr #pre #post (b:bool) (f : unit -> RWI int RW pre post) (g : unit -> RWI int RO pre post) : RWI int RO pre post = if b then f () else g ()
 
-// explodes
-//[@@expect_failure]
-//let test #a #i (n:int) : GTD nat i =
-//  let r = app abs n in
-//  r
+let test_wrw #pre #post (b:bool) (f : unit -> RWI int RW pre post) (g : unit -> RWI int RO pre post) : RWI int RW pre post = if b then f () else g ()
 
-let labs0 #i (n:int) : RWI int i =
+[@@expect_failure]
+let test_wwr #pre #post (b:bool) (f : unit -> RWI int RW pre post) (g : unit -> RWI int RW pre post) : RWI int RO pre post = if b then f () else g ()
+
+let test_www #pre #post (b:bool) (f : unit -> RWI int RW pre post) (g : unit -> RWI int RW pre post) : RWI int RW pre post = if b then f () else g ()
+
+// EXPLODES: bound term variable not found in env...
+//let rec map #a #b
+//  (f : a -> RWI b RO (fun _ -> True) (fun _ _ _ -> True))
+//  (xs : list a)
+//  : RWI (list b) RO (fun _ -> True) (fun _ _ _ -> True)
+//  = match xs with
+//    | [] -> []
+//    | x::xs -> (f x)::(map #_ #_ f xs)
+
+let app #a #b #i #pre #post (f : a -> RWI b i pre post) (x : a) : RWI b i pre post = f x
+
+// can't resolve an index, providing it explicitly with #i makes it explode too
+//let rec appn #a #i (n:nat) (f : a -> RWI a i (fun _ -> True) (fun _ _ _ -> True)) (x : a) : RWI a i (fun _ -> True)
+//(fun _ _ _ -> True) =
+//  match n with 
+//  | 0 -> x
+//  | _ -> begin
+//    //assume (n>0);
+//    appn #a #i (n-1) f (f x)
+//  end
+
+let labs0 (n:int) : RWI int RO (fun _ -> True) (fun h0 x h1 -> x >= 0 /\ h1 == h0) =
   if n < 0
   then -n
   else n
+
+let labs (n:int) : RWI nat RO (fun _ -> True) (fun h0 _ h1 -> True) =
+  if n < 0
+  then -n
+  else n
+
+let rwi_assert (p:Type0) : RWI unit RO (fun _ -> p) (fun h0 () h1 -> h0 == h1) =
+  // assert p // fails
+  RWI?.reflect (fun () -> assert p)
   
-let labs #i (n:int) : RWI nat i =
-  if n < 0
-  then -n
-  else n
+let rwi_assume (p:Type0) : RWI unit RO (fun _ -> True) (fun h0 () h1 -> h0 == h1 /\ p) =
+  RWI?.reflect (fun () -> assume p)
 
-[@@expect_failure]
-let test #a #i (n:int) : RWI nat i =
+let test_abs0 (n:int) : RWI int RO (fun _ -> True) (fun h0 r h1 -> r >= 0) =
   let r = labs0 n in
-  assume (r >= 0);
+  ();
+  ();
+  r
+  
+let test_abs0' (n:int) : RWI nat RO (fun _ -> True) (fun h0 _ h1 -> True) =
+  let r = labs0 n in
+  let r : nat = r in // need this! an ascription won't work!
+  r
+  
+let test_abs (n:int) : RWI nat RO (fun _ -> True) (fun h0 _ h1 -> True) =
+  let r = labs n in
   r
 
-let getr () : RWI H.heap R =
-  RWI?.reflect begin
-    let f' () : ST H.heap (fun _ -> True) (fun h0 _ h1 -> h0 == h1) = get () in
-    pack_r f'
-  end
+// just a test
+let get_indexed (#i:idx) () : RWI H.heap i (fun _ -> True) (fun h0 x h1 -> x == h0 /\ h1 == h0) =
+  RWI?.reflect (fun () -> ST.get ())
 
-let get (#i:idx) () : RWI H.heap i =
-  RWI?.reflect begin
-    match i with
-    | R ->
-      let f' () : ST H.heap (fun _ -> True) (fun h0 _ h1 -> h0 == h1) = get () in
-      pack_r f'
+let get_r () : RWI H.heap RO (fun _ -> True) (fun h0 x h1 -> x == h0 /\ h1 == h0) =
+  RWI?.reflect (fun () -> ST.get ())
 
-    | RW ->
-      let f' () : ST H.heap (fun _ -> True) (fun _ _ _ -> True) = get () in
-      pack_rw f'
-  end
+//let get #i = get_indexed #i
+let get = get_r
+
+let test_state_eq_rrr
+  (f g : unit -> RWI int RO (fun _ -> True) (fun _ _ _ -> True))
+  : RWI int RO (fun _ -> True) (fun _ _ _ -> True)
+  =
+  let h0 = get () in
+  let x = f () in
+  let h1 = get () in
+  let y = g () in
+  let h2 = get () in
+  assert (h0 == h1);
+  assert (h1 == h2);
+  x + y
+  
+let test_state_eq_rrw
+  (f : unit -> RWI int RO (fun _ -> True) (fun _ _ _ -> True))
+  (g : unit -> RWI int RO (fun _ -> True) (fun _ _ _ -> True))
+  : RWI int RW (fun _ -> True) (fun _ _ _ -> True)
+  =
+  let h0 = get () in
+  let x = f () in
+  let h1 = get () in
+  let y = g () in
+  let h2 = get () in
+  assert (h0 == h1);
+  assert (h1 == h2);
+  x + y
+
+let test_state_eq_rww
+  (f : unit -> RWI int RO (fun _ -> True) (fun _ _ _ -> True))
+  (g : unit -> RWI int RW (fun _ -> True) (fun _ _ _ -> True))
+  : RWI int RW (fun _ -> True) (fun _ _ _ -> True)
+  =
+  let h0 = get () in
+  let x = f () in
+  let h1 = get () in
+  let y = g () in
+  let h2 = get () in
+  assert (h0 == h1);
+  x + y
+
+let test_state_eq_www
+  (f : unit -> RWI int RW (fun _ -> True) (fun _ _ _ -> True))
+  (g : unit -> RWI int RW (fun _ -> True) (fun _ _ _ -> True))
+  : RWI int RW (fun _ -> True) (fun _ _ _ -> True)
+  =
+  let h0 = get () in
+  let x = f () in
+  let h1 = get () in
+  let y = g () in
+  let h2 = get () in
+  //assert (h0 == h1);
+  //assert (h1 == h2);
+  x + y
